src/coq/Imp.v
@@ -1306,6 +1306,8 @@ Reserved Notation "c1 '/' st1 '==>' co '/' st2"
 Reserved Notation "c1 '/' st1 '==>' - '/' st2"
          (at level 40, st1 at level 39, st2 at level 38).
 
+Hint Constructors ceval.
+
 Inductive ceval_small : com -> state -> (option com) -> state -> Prop :=
 | S_Skip : forall st,
              SKIP / st ==> - / st
@@ -1342,8 +1344,106 @@ Inductive ceval_small : com -> state -> (option com) -> state -> Prop :=
   and "c1 '/' st1 '==>' - '/' st2"  := (ceval_small c1 st1 None st2)
 .             
 
+Hint Constructors ceval_small.
 
+Inductive ceval_small_N : nat -> com -> state -> state -> Prop :=
+| small0 : forall c st1 st2,
+    c / st1 ==> - / st2 ->
+    ceval_small_N 0 c st1 st2
+| smallS : forall n c1 c2 st1 st2 st3,
+    c1 / st1 ==> c2 / st2 ->
+    ceval_small_N n c2 st2 st3 ->
+    ceval_small_N (S n) c1 st1 st3
+.
+Hint Constructors ceval_small_N.
 
+Lemma ceval_small_seq : forall c1 c2 st1 st2 st3 n1 n2,
+    ceval_small_N n1 c1 st1 st2 ->
+    ceval_small_N n2 c2 st2 st3 ->
+    ceval_small_N (1+(n1+n2)) (c1 ;; c2) st1 st3.
+Proof.
+  intros c1 c2 st1 st2 st3 n1 n2 H12.
+  revert c2 st3 n2.
+  induction H12; intros c2' st3' n2' H23.
+  - simpl. eauto.
+  - apply smallS with (c2:=(c2;;c2'))(st2:=st2). apply S_Seq1. apply H.
+    apply IHceval_small_N. exact H23.
+Qed.    
+
+Lemma ceval_big_small : forall c st1 st2,
+    c / st1 \\ st2 -> exists n, ceval_small_N n c st1 st2.
+Proof.
+  intros c st1 st2 H.
+  induction H.
+  - exists 0; auto.
+  - exists 0; auto.
+  - destruct IHceval1 as [n1 Hsm1].
+    destruct IHceval2 as [n2 Hsm2].
+    exists (1+(n1+n2)). eapply ceval_small_seq; eauto.
+  - destruct IHceval as [n1 Hsm1].
+    exists (1+n1). eauto.
+  - destruct IHceval as [n1 Hsm1].
+    exists (1+n1). eauto.
+  - exists 0; auto.
+  - destruct IHceval1 as [n1 Hsm1].
+    destruct IHceval2 as [n2 Hsm2].
+    exists (2+(n1+n2)). eapply smallS. eauto.
+    eapply ceval_small_seq; eauto.
+Qed.
+
+Lemma ceval_assoc : forall c1 c2 c3 s s',
+    (c1 ;; (c2 ;; c3)) / s \\ s' <->
+    ((c1 ;; c2) ;; c3) / s \\ s'.
+Proof.
+  intros c1 c2 c3 s s'.
+  split; intros H.
+  - inversion H; subst.
+    inversion H5; subst.
+    eauto.
+  - inversion H; subst.
+    inversion H2; subst.
+    eauto.
+Qed.  
+
+Lemma ceval_small_big : forall c1 c2 c3 st1 st2 st3
+    (Hs : c1 / st1 ==> c2 / st2)
+    (Hbig : (c2 ;; c3) / st2 \\ st3),
+    (c1 ;; c3) / st1 \\ st3.
+Proof.
+  induction c1; intros c2 c3 st1 st2 st3 Hs Hbig; try solve [inversion Hs].
+  - inversion Hs; subst.
+    + apply ceval_assoc.
+      apply ceval_assoc in Hbig.
+      eapply IHc1_1. apply H4. apply Hbig.
+    + apply ceval_assoc.
+      inversion H4; subst.
+      * eapply E_Seq; eauto.
+      * eapply E_Seq; eauto. eauto.
+      * eapply E_Seq; eauto.
+  - inversion Hs; subst.
+    + inversion Hbig; subst.
+      eapply E_Seq; eauto.
+    + inversion Hbig; subst.
+      eapply E_Seq; eauto.
+  - inversion Hs; subst.
+    inversion Hbig; subst.
+    inversion H1. subst.
+    eapply E_Seq.
+    eapply E_WhileLoop; eauto. apply H5.
+Qed.    
+    
+Lemma ceval_small_N_ceval : forall n c st1 st2,
+    ceval_small_N n c st1 st2 -> c / st1 \\ st2.
+Proof.
+  intros n c st1 st2 H.
+  induction H.
+  - inversion H; subst; auto.
+  - inversion H; subst; auto.
+    eapply ceval_small_big; eauto.
+    inversion H4; subst; eapply E_Seq; eauto. eauto.
+    inversion IHceval_small_N. subst.
+    eapply E_WhileLoop; eauto.
+Qed.    
 
 
 (** The cost of defining evaluation as a relation instead of a
